src/dvspec/dafny/att_spec_proofs/dvn_next_invs_19.dfy
@@ -1,0 +1,139 @@
+include "../commons.dfy"
+include "../specification/dvc_spec.dfy"
+include "../specification/consensus.dfy"
+include "../specification/network.dfy"
+include "../specification/dvn.dfy"
+include "../att_spec_proofs/inv.dfy"
+include "../att_spec_proofs/assump.dfy"
+include "../att_spec_proofs/fnc_inv.dfy"
+include "../att_spec_proofs/helper_sets_lemmas.dfy"
+include "../att_spec_proofs/proofs_intermediate_steps.dfy"
+include "../att_spec_proofs/dvn_next_invs_1_7.dfy"
+include "../att_spec_proofs/dvn_next_invs_8_18.dfy"
+
+module DVN_Next_Invs_19
+{
+    import opened Types 
+    import opened CommonFunctions
+    import opened ConsensusSpec
+    import opened NetworkSpec
+    import opened DVCNode_Spec
+    import opened DV
+    import opened Att_Inv_With_Empty_Initial_Attestation_Slashing_DB
+    import opened Att_Assumptions
+    import opened Fnc_Inv
+    import opened Helper_Sets_Lemmas
+    import opened Proofs_Intermediate_Steps
+    import opened DVN_Next_Invs_1_7
+    import opened DVN_Next_Invs_8_18
+
+    lemma lemma_inv19_dvn_next(
+        dvn: DVState,
+        event: DV.Event,
+        dvn': DVState
+    )    
+    requires NextEvent(dvn, event, dvn')    
+    requires inv19(dvn')    
+    ensures inv19(dvn')    
+    { }
+
+    lemma lemma_inv20_dvn_next(
+        dvn: DVState,
+        event: DV.Event,
+        dvn': DVState
+    )    
+    requires NextEvent(dvn, event, dvn')    
+    ensures inv20(dvn, dvn')
+    { }
+
+    lemma lemma_inv21_dvn_next(
+        dvn: DVState,
+        event: DV.Event,
+        dvn': DVState
+    )
+    requires inv1(dvn)    
+    requires NextEvent(dvn, event, dvn')
+    requires inv20(dvn, dvn')
+    requires inv21(dvn)
+    ensures inv21(dvn')
+    {        
+        match event 
+        {
+            case HonestNodeTakingStep(node, nodeEvent, nodeOutputs) =>
+                var dvc := dvn.honest_nodes_states[node];
+                var dvc' := dvn'.honest_nodes_states[node];
+                match nodeEvent
+                {
+                    case ServeAttstationDuty(att_duty) =>     
+                        var index := dvn.index_next_attestation_duty_to_be_served;
+                        var new_duty := dvn.sequence_attestation_duties_to_be_served[index].attestation_duty;                                
+                        lemma_inv4_f_serve_attestation_duty(dvc, new_duty, dvc');    
+                        assert dvc'.all_rcvd_duties == dvc.all_rcvd_duties + {new_duty};                                                                                                       
+                        var new_index := dvn'.index_next_attestation_duty_to_be_served;
+                        assert index + 1 == new_index;
+                        
+                        forall k: nat | ( && 0 <= k < new_index
+                                          && dvn'.sequence_attestation_duties_to_be_served[k].node in dvn'.honest_nodes_states.Keys
+                                        )    
+                        ensures index + 1 == new_index
+                        ensures dvn'.sequence_attestation_duties_to_be_served[k].attestation_duty
+                                    in dvn'.honest_nodes_states[dvn'.sequence_attestation_duties_to_be_served[k].node].all_rcvd_duties                            
+                        {
+                            var duty_and_node: AttestationDutyAndNode := dvn.sequence_attestation_duties_to_be_served[k];
+                            var duty := duty_and_node.attestation_duty;
+                            var hn := duty_and_node.node;
+                            var dvc_state := dvn.honest_nodes_states[hn];
+                            var dvc_state' := dvn'.honest_nodes_states[hn];
+
+                            if hn == node
+                            {
+                                if k < index
+                                {     
+                                    assert inv21_body(dvc_state, duty);
+                                    assert inv21_body(dvc_state', duty);
+                                }
+                                else
+                                {
+                                    assert k == index;
+                                    assert k == new_index - 1;
+                                    lemma_inv4_f_serve_attestation_duty(dvc_state, att_duty, dvc_state');                                
+                                    assert dvc'.all_rcvd_duties == dvc.all_rcvd_duties + {att_duty};
+                                    assert att_duty in dvc'.all_rcvd_duties;                                
+                                    assert inv21_body(dvc_state', duty);
+                                }
+                            }
+                            else
+                            {
+                                assert dvc_state == dvc_state';
+                                assert inv21_body(dvc_state', duty);
+                            }
+                            
+                            assert inv21_body(dvc_state', duty);
+                        }
+                        
+                        assert inv21(dvn');
+
+                    case AttConsensusDecided(id, decided_attestation_data) => 
+                        lemma_inv4_f_att_consensus_decided(dvc, id, decided_attestation_data, dvc');                        
+                        
+                    case ReceviedAttesttionShare(attestation_share) =>                         
+                        lemma_inv4_f_listen_for_attestation_shares(dvc, attestation_share, dvc');                        
+   
+                    case ImportedNewBlock(block) => 
+                        var dvc := add_block_to_bn(dvc, nodeEvent.block);
+                        lemma_inv4_f_listen_for_new_imported_blocks(dvc, block, dvc');                        
+                                                
+                    case ResendAttestationShares =>                         
+                        
+                    case NoEvent => 
+                        
+                }
+
+            case AdeversaryTakingStep(node, new_attestation_share_sent, messagesReceivedByTheNode) =>
+                
+        }        
+    }   
+    
+    
+}   
+        
