src/dvspec/dafny/specification/dvn.dfy
@@ -203,9 +203,9 @@ module DV
         )
         && (forall i: Slot :: i in s.consensus_on_attestation_data 
                             ==> !s.consensus_on_attestation_data[i].decided_value.isPresent()
-        )
+        )        
         && is_sequence_attestation_duties_to_be_served_orders(s)
-        
+        && s.index_next_attestation_duty_to_be_served == 0        
     }
 
     predicate is_sequence_attestation_duties_to_be_served_orders(s: DVState)
